share/pulse/examples/dice/cbor/COSE.AST.fst
@@ -5,48 +5,45 @@ module Spec = COSE.Spec
 #push-options "--fuel 0"
 
 [@@ bounded_attr; sem_attr]
-let e0 = empty_env
-let thr0 : spec_array_group_splittable_threshold e0 = spec_array_group_splittable_threshold_empty _
+let e0 = empty_wf_ast_env
 
 [@@ bounded_attr; sem_attr]
-let e1 = env_extend_map_group e0 "header_map0" 
-  (_ by (solve_env_extend_array_group ()))
+let e1 = wf_ast_env_extend_map_group e0 "header_map0" 
+  (_ by (solve_bounded ()))
   Spec.header_map0
-  (_ by (solve_env_extend_array_group ()))
+  (_ by (solve_bounded ()))
+  (_ by (solve_spec_ast_env_elem_well_formed ()))
 
 [@@ bounded_attr; sem_attr]
-let e2 = env_extend_typ e1 "header_map"
-  (_ by (solve_env_extend_array_group ()))
+let e2 = wf_ast_env_extend_typ e1 "header_map"
+  (_ by (solve_bounded ()))
   (TElem (TMap "header_map0"))
-  (_ by (solve_env_extend_array_group ()))
+  (_ by (solve_bounded ()))
+  (_ by (solve_spec_ast_env_elem_well_formed ()))
 
 [@@ bounded_attr; sem_attr]
-let e3 = env_extend_typ e2 "empty_or_serialized_map"
-  (_ by (solve_env_extend_array_group ()))
+let e3 = wf_ast_env_extend_typ e2 "empty_or_serialized_map"
+  (_ by (solve_bounded ()))
   (TEscapeHatch Spec.empty_or_serialized_map)
-  (_ by (solve_env_extend_array_group ()))
+  (_ by (solve_bounded ()))
+  (_ by (solve_spec_ast_env_elem_well_formed ()))
 
 [@@ bounded_attr; sem_attr]
 let e4 =
-  env_extend_array_group e3 "headers"
-    (_ by (solve_env_extend_array_group ()))
+  wf_ast_env_extend_array_group e3 "headers"
+    (_ by (solve_bounded ()))
     [
       "protected", TAAtom (TAElem (TDef "empty_or_serialized_map"));
       "unprotected", TAAtom (TAElem (TDef "header_map"));
     ]
-    (_ by (solve_env_extend_array_group ()))
-
-let thr4 : spec_array_group_splittable_threshold e4 =
-  spec_array_group_splittable_threshold_extend
-    (spec_array_group_splittable_threshold_extend_env thr0 e4)
-    "headers"
-    (_ by (solve_spec_array_group_splittable ()))
+    (_ by (solve_bounded ()))
+    (_ by (solve_spec_ast_env_elem_well_formed ()))
 
 let _ : squash (
-  se_array_group e4.e_semenv "headers" `CDDL.Spec.array_group3_equiv` Spec.headers
+  se_array_group e4.we_env.e_semenv "headers" `CDDL.Spec.array_group3_equiv` Spec.headers
 ) = 
-  let a = normalize_term (e4.e_env "headers") in
-  assert (array_group_sem e4.e_semenv a `CDDL.Spec.array_group3_equiv` Spec.headers)
+  let a = (e4.we_env.e_env "headers") in
+  assert (array_group_sem e4.we_env.e_semenv a `CDDL.Spec.array_group3_equiv` Spec.headers)
     by (solve_sem_equiv ())
 
 [@@ bounded_attr; sem_attr]
@@ -54,41 +51,35 @@ let e5 = e4
 
 [@@ bounded_attr; sem_attr]
 let e6 =
-  env_extend_typ e5 "cose_signature"
-    (_ by (solve_env_extend_array_group ()))
+  wf_ast_env_extend_typ e5 "cose_signature"
+    (_ by (solve_bounded ()))
     (TArray [
       "headers", TAAtom (TADef "headers");
       "signature", TAAtom (TAElem (TByteString));
     ])
-    (_ by (solve_env_extend_array_group ()))
-
-(* // TODO: type well-formedness, i.e. inner array type splittable 
-let thr6 : spec_array_group_splittable_threshold e6 =
-  spec_array_group_splittable_threshold_extend
-    (spec_array_group_splittable_threshold_extend_env thr4 e6)
-    "cose_signature_array"
-    (_ by (solve_spec_array_group_splittable ()))
-*)
+    (_ by (solve_bounded ()))
+    (_ by (solve_spec_ast_env_elem_well_formed ()))
 
 [@@ bounded_attr; sem_attr]
 let e7 = e6
 
 let _ : squash (
-  se_typ e7.e_semenv "cose_signature" `CDDL.Spec.typ_equiv` Spec.cose_signature
+  se_typ e7.we_env.e_semenv "cose_signature" `CDDL.Spec.typ_equiv` Spec.cose_signature
 ) = 
-  let a = normalize_term (e7.e_env "cose_signature") in
-  assert (typ_sem e7.e_semenv a `CDDL.Spec.typ_equiv` Spec.cose_signature)
+  let a = (e7.we_env.e_env "cose_signature") in
+  assert (typ_sem e7.we_env.e_semenv a `CDDL.Spec.typ_equiv` Spec.cose_signature)
     by (solve_sem_equiv ())
 
 [@@ bounded_attr; sem_attr]
 let e8 =
-  env_extend_typ e7 "cose_sign_payload" 
-    (_ by (solve_env_extend_array_group ()))
+  wf_ast_env_extend_typ e7 "cose_sign_payload" 
+    (_ by (solve_bounded ()))
     (TChoice [
       TByteString;
       TNil;
     ])
-    (_ by (solve_env_extend_array_group ()))
+    (_ by (solve_bounded ()))
+    (_ by (solve_spec_ast_env_elem_well_formed ()))
 
 [@@ bounded_attr; sem_attr]
 let e9 = e8
@@ -96,50 +87,44 @@ let e9 = e8
 [@@ bounded_attr; sem_attr]
 let e10 = e9
 
-(* // TODO
-let thr10 : spec_array_group_splittable_threshold e10 =
-  spec_array_group_splittable_threshold_extend
-    (spec_array_group_splittable_threshold_extend_env thr9 e10)
-    "cose_sign_array"
-    (_ by (solve_spec_array_group_splittable ()))
-*)
-
 [@@ bounded_attr; sem_attr]
 let e11 =
-  env_extend_typ e10 "cose_sign"
-    (_ by (solve_env_extend_array_group ()))
+  wf_ast_env_extend_typ e10 "cose_sign"
+    (_ by (solve_bounded ()))
     (TArray [
       "headers", TAAtom (TADef "headers");
       "payload", TAAtom (TAElem (TDef "cose_sign_payload"));
       "signatures", TAAtom (TAElem (TElemArray (TAOneOrMore (TAElem (TDef "cose_signature")))));
     ])
-    (_ by (solve_env_extend_array_group ()))
+    (_ by (solve_bounded ()))
+    (_ by (solve_spec_ast_env_elem_well_formed ()))
 
 #push-options "--z3rlimit 16" // cannot reason about typ_equiv
 
 let _ : squash (
-  se_typ e11.e_semenv "cose_sign" `CDDL.Spec.typ_equiv` Spec.cose_sign
+  se_typ e11.we_env.e_semenv "cose_sign" `CDDL.Spec.typ_equiv` Spec.cose_sign
 ) = 
-  let a = normalize_term (e11.e_env "cose_sign") in
-  assert (typ_sem e11.e_semenv a `CDDL.Spec.typ_equiv` Spec.cose_sign)
+  let a = (e11.we_env.e_env "cose_sign") in
+  assert (typ_sem e11.we_env.e_semenv a `CDDL.Spec.typ_equiv` Spec.cose_sign)
     by (solve_sem_equiv ())
 
 #pop-options
 
 [@@ bounded_attr; sem_attr]
 let e12 =
-  env_extend_typ e11 "cose_sign_tagged"
-    (_ by (solve_env_extend_array_group ()))
+  wf_ast_env_extend_typ e11 "cose_sign_tagged"
+    (_ by (solve_bounded ()))
     (TTag Spec.tag_cose_sign (TDef "cose_sign"))
-    (_ by (solve_env_extend_array_group ()))
+    (_ by (solve_bounded ()))
+    (_ by (solve_spec_ast_env_elem_well_formed ()))
 
 #push-options "--z3rlimit 16" // cannot reason about typ_equiv
 
 let _ : squash (
-  se_typ e12.e_semenv "cose_sign_tagged" `CDDL.Spec.typ_equiv` Spec.cose_sign_tagged
+  se_typ e12.we_env.e_semenv "cose_sign_tagged" `CDDL.Spec.typ_equiv` Spec.cose_sign_tagged
 ) = 
-  let a = normalize_term (e12.e_env "cose_sign_tagged") in
-  assert (typ_sem e12.e_semenv a `CDDL.Spec.typ_equiv` Spec.cose_sign_tagged)
+  let a = (e12.we_env.e_env "cose_sign_tagged") in
+  assert (typ_sem e12.we_env.e_semenv a `CDDL.Spec.typ_equiv` Spec.cose_sign_tagged)
     by (solve_sem_equiv ())
 
 #pop-options
@@ -147,50 +132,44 @@ let _ : squash (
 [@@ bounded_attr; sem_attr]
 let e13 = e12
 
-(* // TODO
-let thr13 : spec_array_group_splittable_threshold e13 =
-  spec_array_group_splittable_threshold_extend
-    (spec_array_group_splittable_threshold_extend_env thr10 e13)
-    "cose_sign1_array"
-    (_ by (solve_spec_array_group_splittable ()))
-*)
-
 [@@ bounded_attr; sem_attr]
 let e14 =
-  env_extend_typ e13 "cose_sign1"
-    (_ by (solve_env_extend_array_group ()))
+  wf_ast_env_extend_typ e13 "cose_sign1"
+    (_ by (solve_bounded ()))
     (TArray [
       "headers", TAAtom (TADef "headers");
       "payload", TAAtom (TAElem (TDef "cose_sign_payload"));
       "signature", TAAtom (TAElem TByteString);
     ])
-    (_ by (solve_env_extend_array_group ()))
+    (_ by (solve_bounded ()))
+    (_ by (solve_spec_ast_env_elem_well_formed ()))
 
 #push-options "--z3rlimit 16" // cannot reason about typ_equiv
 
 let _ : squash (
-  se_typ e14.e_semenv "cose_sign1" `CDDL.Spec.typ_equiv` Spec.cose_sign1
+  se_typ e14.we_env.e_semenv "cose_sign1" `CDDL.Spec.typ_equiv` Spec.cose_sign1
 ) = 
-  let a = normalize_term (e14.e_env "cose_sign1") in
-  assert (typ_sem e14.e_semenv a `CDDL.Spec.typ_equiv` Spec.cose_sign1)
+  let a = e14.we_env.e_env "cose_sign1" in
+  assert (typ_sem e14.we_env.e_semenv a `CDDL.Spec.typ_equiv` Spec.cose_sign1)
     by (solve_sem_equiv ())
 
 #pop-options
 
 [@@ bounded_attr; sem_attr]
 let e15 =
-  env_extend_typ e14 "cose_sign1_tagged"
-    (_ by (solve_env_extend_array_group ()))
+  wf_ast_env_extend_typ e14 "cose_sign1_tagged"
+    (_ by (solve_bounded ()))
     (TTag Spec.tag_cose_sign1 (TDef "cose_sign1"))
-    (_ by (solve_env_extend_array_group ()))
+    (_ by (solve_bounded ()))
+    (_ by (solve_spec_ast_env_elem_well_formed ()))
 
 #push-options "--z3rlimit 16" // cannot reason about typ_equiv
 
 let _ : squash (
-  se_typ e15.e_semenv "cose_sign1_tagged" `CDDL.Spec.typ_equiv` Spec.cose_sign1_tagged
+  se_typ e15.we_env.e_semenv "cose_sign1_tagged" `CDDL.Spec.typ_equiv` Spec.cose_sign1_tagged
 ) = 
-  let a = normalize_term (e15.e_env "cose_sign1_tagged") in
-  assert (typ_sem e15.e_semenv a `CDDL.Spec.typ_equiv` Spec.cose_sign1_tagged)
+  let a = (e15.we_env.e_env "cose_sign1_tagged") in
+  assert (typ_sem e15.we_env.e_semenv a `CDDL.Spec.typ_equiv` Spec.cose_sign1_tagged)
     by (solve_sem_equiv ())
 
 #pop-options
